zoo_saturn/mpsc_queue_1: Rewrite.

theories/zoo_saturn/mpsc_queue_1.v
@@ -24,9 +24,9 @@ From zoo Require Import
   options.
 
 Implicit Types b : bool.
-Implicit Types l front node back new_back : location.
+Implicit Types front node back new_back : location.
 Implicit Types hist past nodes : list location.
-Implicit Types v t : val.
+Implicit Types v : val.
 Implicit Types o : option val.
 Implicit Types vs : list val.
 
@@ -46,126 +46,800 @@ Proof.
   solve_inG.
 Qed.
 
+Module base.
+  Section mpsc_queue_1_G.
+    Context `{mpsc_queue_1_G : MpscQueue1G Σ}.
+
+    Implicit Types t : location.
+
+    Record mpsc_queue_1_name := {
+      mpsc_queue_1_name_inv : namespace ;
+      mpsc_queue_1_name_history : gname ;
+      mpsc_queue_1_name_model : gname ;
+    }.
+    Implicit Type γ : mpsc_queue_1_name.
+
+    #[global] Instance mpsc_queue_1_name_eq_dec : EqDecision mpsc_queue_1_name :=
+      ltac:(solve_decision).
+    #[global] Instance mpsc_queue_1_name_countable :
+      Countable mpsc_queue_1_name.
+    Proof.
+      solve_countable.
+    Qed.
+
+    #[local] Definition history_auth' γ_history hist :=
+      mono_list_auth γ_history (DfracOwn 1) hist.
+    #[local] Definition history_auth γ hist :=
+      history_auth' γ.(mpsc_queue_1_name_history) hist.
+    #[local] Definition history_at γ i node :=
+      mono_list_at γ.(mpsc_queue_1_name_history) i node.
+
+    #[local] Definition model₁' γ_model vs :=
+      twins_twin1 γ_model (DfracOwn 1) vs.
+    #[local] Definition model₁ γ vs :=
+      model₁' γ.(mpsc_queue_1_name_model) vs.
+    #[local] Definition model₂' γ_model vs :=
+      twins_twin2 γ_model vs.
+    #[local] Definition model₂ γ vs :=
+      model₂' γ.(mpsc_queue_1_name_model) vs.
+
+    #[local] Definition node_model γ node i : iProp Σ :=
+      node ↦ₕ Header §Node 2 ∗
+      history_at γ i node.
+    #[local] Instance : CustomIpatFormat "node_model" :=
+      " ( #H{}_header &
+          #Hhistory_at_{}
+        )
+      ".
+
+    #[local] Definition inv_inner t γ : iProp Σ :=
+      ∃ hist past front nodes back vs,
+      ⌜hist = past ++ front :: nodes⌝ ∗
+      ⌜back ∈ hist⌝ ∗
+      t.[front] ↦{#1/4} #front ∗
+      t.[back] ↦ #back ∗
+      xtchain (Header §Node 2) (DfracOwn 1) hist §Null ∗
+      ([∗ list] node; v ∈ nodes; vs, node.[data] ↦ v) ∗
+      history_auth γ hist ∗
+      model₂ γ vs.
+    #[local] Instance : CustomIpatFormat "inv_inner" :=
+      " ( %hist{} &
+          %past{} &
+          %front{} &
+          %nodes{} &
+          %back{} &
+          %vs{} &
+          >%Hhist{} &
+          >%Hback{} &
+          >Ht_front &
+          >Ht_back &
+          >Hhist &
+          >Hnodes &
+          >Hhistory_auth &
+          >Hmodel₂
+        )
+      ".
+    #[local] Definition inv' t γ :=
+      inv γ.(mpsc_queue_1_name_inv) (inv_inner t γ).
+    Definition mpsc_queue_1_inv t γ ι : iProp Σ :=
+      ⌜ι = γ.(mpsc_queue_1_name_inv)⌝ ∗
+      inv' t γ.
+    #[local] Instance : CustomIpatFormat "inv" :=
+      " ( -> &
+          #Hinv
+        )
+      ".
+
+    Definition mpsc_queue_1_model :=
+      model₁.
+    #[local] Instance : CustomIpatFormat "model" :=
+      " Hmodel₁{_{}}
+      ".
+
+    #[local] Definition consumer_1 t front : iProp Σ :=
+      t.[front] ↦{#3/4} #front.
+    #[local] Definition consumer_2 t : iProp Σ :=
+      ∃ front,
+      consumer_1 t front.
+    #[local] Instance : CustomIpatFormat "consumer_2" :=
+      " ( %front{} &
+          Hconsumer{_{}}
+        )
+      ".
+    Definition mpsc_queue_1_consumer :=
+      consumer_2.
+    #[local] Instance : CustomIpatFormat "consumer" :=
+      " (:consumer_2 {//})
+      ".
+
+    #[global] Instance mpsc_queue_1_model_timeless γ vs :
+      Timeless (mpsc_queue_1_model γ vs).
+    Proof.
+      apply _.
+    Qed.
+    #[global] Instance mpsc_queue_1_consumer_timeless t :
+      Timeless (mpsc_queue_1_consumer t).
+    Proof.
+      apply _.
+    Qed.
+
+    #[global] Instance mpsc_queue_1_inv_persistent t γ ι :
+      Persistent (mpsc_queue_1_inv t γ ι).
+    Proof.
+      apply _.
+    Qed.
+
+    #[local] Lemma history_alloc front :
+      ⊢ |==>
+        ∃ γ_history,
+        history_auth' γ_history [front].
+    Proof.
+      apply mono_list_alloc.
+    Qed.
+    #[local] Lemma history_at_get {γ hist} i node :
+      hist !! i = Some node →
+      history_auth γ hist ⊢
+      history_at γ i node.
+    Proof.
+      apply mono_list_at_get.
+    Qed.
+    #[local] Lemma history_at_lookup γ hist i node :
+      history_auth γ hist -∗
+      history_at γ i node -∗
+      ⌜hist !! i = Some node⌝.
+    Proof.
+      apply mono_list_at_valid.
+    Qed.
+    #[local] Lemma history_update {γ hist} node :
+      history_auth γ hist ⊢ |==>
+        history_auth γ (hist ++ [node]) ∗
+        history_at γ (length hist) node.
+    Proof.
+      iIntros "Hauth".
+      iMod (mono_list_update_snoc with "Hauth") as "Hauth".
+      iDestruct (history_at_get with "Hauth") as "#Hat".
+      { rewrite lookup_snoc_Some. naive_solver. }
+      iSteps.
+    Qed.
+
+    #[local] Lemma model_alloc :
+      ⊢ |==>
+        ∃ γ_model,
+        model₁' γ_model [] ∗
+        model₂' γ_model [].
+    Proof.
+      apply twins_alloc'.
+    Qed.
+    #[local] Lemma model₁_exclusive γ vs1 vs2 :
+      model₁ γ vs1 -∗
+      model₁ γ vs2 -∗
+      False.
+    Proof.
+      apply twins_twin1_exclusive.
+    Qed.
+    #[local] Lemma model_agree γ vs1 vs2 :
+      model₁ γ vs1 -∗
+      model₂ γ vs2 -∗
+      ⌜vs1 = vs2⌝.
+    Proof.
+      apply: twins_agree_L.
+    Qed.
+    #[local] Lemma model_update {γ vs1 vs2} vs :
+      model₁ γ vs1 -∗
+      model₂ γ vs2 ==∗
+        model₁ γ vs ∗
+        model₂ γ vs.
+    Proof.
+      apply twins_update.
+    Qed.
+
+    #[local] Lemma inv_inner_history_at t γ front :
+      inv' t γ -∗
+      consumer_1 t front ={⊤}=∗
+        ∃ i,
+        consumer_1 t front ∗
+        node_model γ front i.
+    Proof.
+      iIntros "#Hinv Hconsumer".
+      iInv "Hinv" as "(:inv_inner =1)".
+      iDestruct (pointsto_agree with "Ht_front Hconsumer") as %[= ->].
+      assert (hist1 !! (length past1) = Some front) as Hlookup.
+      { rewrite Hhist1 list_lookup_middle //. }
+      iDestruct (xtchain_lookup_header with "Hhist") as "#Hfront_header"; first done.
+      iDestruct (history_at_get (length past1) front with "Hhistory_auth") as "#Hhistory_at_front"; first done.
+      iSplitR "Hconsumer". { iFrameSteps. }
+      iSteps.
+    Qed.
+
+    Lemma mpsc_queue_1_model_exclusive γ vs1 vs2 :
+      mpsc_queue_1_model γ vs1 -∗
+      mpsc_queue_1_model γ vs2 -∗
+      False.
+    Proof.
+      apply model₁_exclusive.
+    Qed.
+
+    Lemma mpsc_queue_1_consumer_exclusive t :
+      mpsc_queue_1_consumer t -∗
+      mpsc_queue_1_consumer t -∗
+      False.
+    Proof.
+      iIntros "(:consumer =1) (:consumer =2)".
+      iDestruct (pointsto_dfrac_ne with "Hconsumer_1 Hconsumer_2") as %?; naive_solver.
+    Qed.
+
+    Lemma mpsc_queue_1_create_spec ι :
+      {{{
+        True
+      }}}
+        mpsc_queue_1_create ()
+      {{{ t γ,
+        RET #t;
+        meta_token t ⊤ ∗
+        mpsc_queue_1_inv t γ ι ∗
+        mpsc_queue_1_model γ [] ∗
+        mpsc_queue_1_consumer t
+      }}}.
+    Proof.
+      iIntros "%Φ _ HΦ".
+
+      wp_rec.
+      wp_block front as "#Hfront_header" "_" "(Hfront_next & _)".
+      wp_block t as "Hmeta" "(Ht_front & Ht_back & _)".
+      iEval (rewrite -Qp.quarter_three_quarter) in "Ht_front".
+      iDestruct "Ht_front" as "(Ht_front & Hconsumer)".
+
+      iMod history_alloc as "(%γ_history & Hhistory_auth)".
+      iMod model_alloc as "(%γ_model & Hmodel₁ & Hmodel₂)".
+
+      pose γ := {|
+        mpsc_queue_1_name_inv := ι ;
+        mpsc_queue_1_name_history := γ_history ;
+        mpsc_queue_1_name_model := γ_model ;
+      |}.
+
+      iApply ("HΦ" $! t γ).
+      iFrameStep.
+      iApply inv_alloc.
+      iExists [front], [], front, [], front, []. iFrameSteps.
+      - rewrite list_elem_of_singleton //.
+      - rewrite xtchain_singleton. iSteps.
+    Qed.
+
+    #[local] Lemma mpsc_queue_1_front_spec t γ :
+      {{{
+        inv' t γ
+      }}}
+        (#t).{front}
+      {{{ front i,
+        RET #front;
+        node_model γ front i
+      }}}.
+    Proof.
+      iIntros "%Φ #Hinv HΦ".
+
+      iInv "Hinv" as "(:inv_inner)".
+      wp_load.
+      assert (hist !! (length past) = Some front) as Hlookup.
+      { rewrite Hhist list_lookup_middle //. }
+      iDestruct (xtchain_lookup_header with "Hhist") as "#Hfront_header"; first done.
+      iDestruct (history_at_get _ front with "Hhistory_auth") as "#Hhistory_at_front"; first done.
+      iSplitR "HΦ". { iFrameSteps. }
+      iSteps.
+    Qed.
+
+    #[local] Lemma back_spec t γ :
+      {{{
+        inv' t γ
+      }}}
+        (#t).{back}
+      {{{ back i,
+        RET #back;
+        node_model γ back i
+      }}}.
+    Proof.
+      iIntros "%Φ #Hinv HΦ".
+
+      iInv "Hinv" as "(:inv_inner)".
+      wp_load.
+      pose proof Hback as (i & Hlookup)%list_elem_of_lookup.
+      iDestruct (xtchain_lookup_header with "Hhist") as "#Hback_header"; first done.
+      iDestruct (history_at_get with "Hhistory_auth") as "#Hhistory_at_back"; first done.
+      iSplitR "HΦ". { iFrameSteps. }
+      iSteps.
+    Qed.
+
+    Inductive operation :=
+      | IsEmpty (Ψ : bool → iProp Σ)
+      | Pop (Ψ : option val → iProp Σ)
+      | Other.
+    Implicit Types op : operation.
+    Inductive operation' :=
+      | IsEmpty'
+      | Pop'
+      | Other'.
+    #[local] Instance operation'_eq_dec : EqDecision operation' :=
+      ltac:(solve_decision).
+    #[local] Coercion operation_to_operation' op :=
+      match op with
+      | IsEmpty _ =>
+          IsEmpty'
+      | Pop _ =>
+          Pop'
+      | Other =>
+          Other'
+      end.
+    #[local] Definition is_empty_au γ (Ψ : bool → iProp Σ) : iProp Σ :=
+      AU <{
+        ∃∃ vs,
+        model₁ γ vs
+      }> @ ⊤ ∖ ↑γ.(mpsc_queue_1_name_inv), ∅ <{
+        model₁ γ vs
+      , COMM
+        Ψ (bool_decide (vs = []))
+      }>.
+    #[local] Definition pop_au γ (Ψ : option val → iProp Σ) : iProp Σ :=
+      AU <{
+        ∃∃ vs,
+        model₁ γ vs
+      }> @ ⊤ ∖ ↑γ.(mpsc_queue_1_name_inv), ∅ <{
+        model₁ γ (tail vs)
+      , COMM
+        Ψ (head vs)
+      }>.
+    #[local] Lemma next_spec_aux op t γ i node :
+      {{{
+        inv' t γ ∗
+        history_at γ i node ∗
+        ( if decide (op = Other' :> operation') then True else
+            consumer_1 t node
+        ) ∗
+        match op with
+        | IsEmpty Ψ =>
+            is_empty_au γ Ψ
+        | Pop Ψ =>
+            pop_au γ Ψ
+        | Other =>
+            True
+        end
+      }}}
+        (#node).{next}
+      {{{ res,
+        RET res;
+        ( if decide (op = Other' :> operation') then True else
+            consumer_1 t node
+        ) ∗
+        ( ⌜res = §Null%V⌝ ∗
+          match op with
+          | IsEmpty Ψ =>
+              Ψ true
+          | Pop Ψ =>
+              Ψ None
+          | Other =>
+              True
+          end
+        ∨ ∃ node',
+          ⌜res = #node'⌝ ∗
+          node_model γ node' (S i) ∗
+          match op with
+          | IsEmpty Ψ =>
+              Ψ false
+          | Pop Ψ =>
+              pop_au γ Ψ
+          | Other =>
+              True
+          end
+        )
+      }}}.
+    Proof.
+      iIntros "%Φ (#Hinv & #Hhistory_at_node & Hop) HΦ".
+
+      iInv "Hinv" as "(:inv_inner)".
+      iDestruct (history_at_lookup with "Hhistory_auth Hhistory_at_node") as %Hlookup.
+      iDestruct (xtchain_lookup_acc with "Hhist") as "(_ & Hnode & Hhist)"; first done.
+      wp_load.
+      iDestruct ("Hhist" with "Hnode") as "Hhist".
+      destruct (hist !! S i) as [node' |] eqn:Hlookup'; simpl.
+
+      - iDestruct (xtchain_lookup_header with "Hhist") as "#Hnode'_header"; first done.
+        iDestruct (history_at_get (S i) with "Hhistory_auth") as "#Hhistory_at_node'"; first done.
+        destruct op; [| iFrameSteps..].
+        iDestruct "Hop" as "(Hconsumer & HΨ)".
+        iDestruct (pointsto_agree with "Ht_front Hconsumer") as %[= <-].
+
+        iMod "HΨ" as "(%vs_ & (:model) & _ & HΨ)".
+        iDestruct (model_agree with "Hmodel₁ Hmodel₂") as %->.
+        iMod ("HΨ" with "Hmodel₁") as "HΨ".
+
+        iAssert ⌜length past = i⌝%I as %Hpast_length.
+        { iDestruct (xtchain_NoDup with "Hhist") as %Hnodup.
+          iPureIntro. eapply NoDup_lookup; try done.
+          rewrite Hhist list_lookup_middle //.
+        }
+        rewrite -(bool_decide_ext _ _ (length_zero_iff_nil _)).
+        iDestruct (big_sepL2_length with "Hnodes") as %<-.
+        rewrite bool_decide_eq_false_2.
+        { apply (f_equal length) in Hhist as Hhist_length.
+          simpl_length/= in Hhist_length.
+          apply lookup_lt_Some in Hlookup'.
+          lia.
+        }
+
+        iSplitR "Hconsumer HΨ HΦ". { iFrameSteps. }
+        iSteps.
+
+      - destruct_decide (op = Other' :> operation').
+        { destruct op; try done. iSteps. }
+        iDestruct "Hop" as "(Hconsumer & HΨ)".
+        iDestruct (pointsto_agree with "Ht_front Hconsumer") as %[= <-].
+
+        iAssert ⌜length past = i⌝%I as %Hpast_length.
+        { iDestruct (xtchain_NoDup with "Hhist") as %Hnodup.
+          iPureIntro. eapply NoDup_lookup; try done.
+          rewrite Hhist list_lookup_middle //.
+        }
+        destruct_decide (length vs = 0) as ->%nil_length_inv | Hvs; last first.
+        { iDestruct (big_sepL2_length with "Hnodes") as %?.
+          exfalso.
+          apply (f_equal length) in Hhist.
+          opose proof* length_lookup_last as Heq; [done.. |].
+          simpl_length/= in Hhist. lia.
+        }
+
+        destruct op; last done.
+
+        + iMod "HΨ" as "(%vs & (:model) & _ & HΨ)".
+          iDestruct (model_agree with "Hmodel₁ Hmodel₂") as %->.
+          iMod ("HΨ" with "Hmodel₁") as "HΨ".
+
+          iSplitR "Hconsumer HΨ HΦ". { iFrameSteps. }
+          iSteps.
+
+        + iMod "HΨ" as "(%vs & Hmodel₁ & _ & HΨ)".
+          iDestruct (model_agree with "Hmodel₁ Hmodel₂") as %->.
+          iMod ("HΨ" with "Hmodel₁") as "HΨ".
+
+          iSplitR "Hconsumer HΨ HΦ". { iFrameSteps. }
+          iSteps.
+    Qed.
+    #[local] Lemma next_spec {t γ i} node :
+      {{{
+        inv' t γ ∗
+        history_at γ i node
+      }}}
+        (#node).{next}
+      {{{ res,
+        RET res;
+          ⌜res = §Null%V⌝
+        ∨ ∃ node',
+          ⌜res = #node'⌝ ∗
+          node_model γ node' (S i)
+      }}}.
+    Proof.
+      iIntros "%Φ (#Hinv & #Hhistory_at_node) HΦ".
+
+      wp_apply (next_spec_aux Other); iSteps.
+    Qed.
+    #[local] Lemma next_spec_is_empty {t γ i node} Ψ :
+      {{{
+        inv' t γ ∗
+        history_at γ i node ∗
+        consumer_1 t node ∗
+        is_empty_au γ Ψ
+      }}}
+        (#node).{next}
+      {{{ res,
+        RET res;
+        consumer_1 t node ∗
+        ( ⌜res = §Null%V⌝ ∗
+          Ψ true
+        ∨ ∃ node',
+          ⌜res = #node'⌝ ∗
+          node_model γ node' (S i) ∗
+          Ψ false
+        )
+      }}}.
+    Proof.
+      iIntros "%Φ (#Hinv & #Hhistory_at_node & Ht_front & Hau) HΦ".
+
+      wp_apply (next_spec_aux (IsEmpty _) with "[$]").
+      iFrameSteps.
+    Qed.
+    #[local] Lemma next_spec_pop {t γ i node} Ψ :
+      {{{
+        inv' t γ ∗
+        history_at γ i node ∗
+        consumer_1 t node ∗
+        pop_au γ Ψ
+      }}}
+        (#node).{next}
+      {{{ res,
+        RET res;
+        consumer_1 t node ∗
+        ( ⌜res = §Null%V⌝ ∗
+          Ψ None
+        ∨ ∃ node',
+          ⌜res = #node'⌝ ∗
+          node_model γ node' (S i) ∗
+          pop_au γ Ψ
+        )
+      }}}.
+    Proof.
+      iIntros "%Φ (#Hinv & #Hhistory_at_node & Ht_front & Hau) HΦ".
+
+      wp_apply (next_spec_aux (Pop _) with "[$]").
+      iFrameSteps.
+    Qed.
+
+    Lemma mpsc_queue_1_is_empty_spec t γ ι :
+      <<<
+        mpsc_queue_1_inv t γ ι ∗
+        mpsc_queue_1_consumer t
+      | ∀∀ vs,
+        mpsc_queue_1_model γ vs
+      >>>
+        mpsc_queue_1_is_empty #t @ ↑ι
+      <<<
+        mpsc_queue_1_model γ vs
+      | RET #(bool_decide (vs = []%list));
+        mpsc_queue_1_consumer t
+      >>>.
+    Proof.
+      iIntros "%Φ ((:inv) & (:consumer)) HΦ".
+
+      iMod (inv_inner_history_at with "Hinv Hconsumer") as "(%i & Ht_front & #Hfront_header & #Hhistory_at_front)".
+
+      wp_rec. wp_load. wp_match.
+      wp_smart_apply (next_spec_is_empty (λ b, _ -∗ Φ #b)%I with "[$]").
+      iSteps.
+    Qed.
+
+    #[local] Lemma mpsc_queue_1_push_0_spec t γ i node new_back v :
+      <<<
+        inv' t γ ∗
+        node_model γ node i ∗
+        new_back ↦ₕ Header §Node 2 ∗
+        new_back.[next] ↦ §Null ∗
+        new_back.[data] ↦ v
+      | ∀∀ vs,
+        mpsc_queue_1_model γ vs
+      >>>
+        mpsc_queue_1_push_0 #node #new_back @ ↑γ.(mpsc_queue_1_name_inv)
+      <<<
+        mpsc_queue_1_model γ (vs ++ [v])
+      | RET ();
+        ∃ j,
+        history_at γ j new_back
+      >>>.
+    Proof.
+      iIntros "%Φ (#Hinv & (:node_model =node) & #Hnew_back_header & Hnew_back_next & Hnew_back_data) HΦ".
+
+      iLöb as "HLöb" forall (i node) "Hnode_header Hhistory_at_node".
+
+      wp_rec. wp_match.
+      wp_smart_apply (next_spec with "[$]") as (res) "[-> | (%node' & -> & (:node_model =node'))]"; last iSteps.
+      wp_pures.
+
+      wp_bind (CAS _ _ _).
+      iInv "Hinv" as "(:inv_inner)".
+      iDestruct (history_at_lookup with "Hhistory_auth Hhistory_at_node") as %Hlookup.
+      iDestruct (xtchain_lookup with "Hhist") as "(Hhist1 & _ & Hnode & Hhist2)"; first done.
+      destruct (hist !! S i) as [node' |] eqn:Hlookup'; simpl.
+
+      - wp_cas as _ | [=].
+        iDestruct (xtchain_lookup_2 with "Hhist1 Hnode_header Hnode Hhist2") as "Hhist"; [done | rewrite Hlookup' // |].
+        iSplitR "Hnew_back_next Hnew_back_data HΦ". { iFrameSteps. }
+        iSteps.
+
+      - wp_cas as ? | _; first done.
+        iDestruct (xtchain_lookup_2 with "Hhist1 Hnode_header Hnode []") as "Hhist"; [done | rewrite Hlookup' // | ..].
+        { rewrite -(length_lookup_last hist i) // drop_all.
+          iApply xtchain_nil.
+        }
+        iDestruct (big_sepL2_snoc_2 with "Hnodes Hnew_back_data") as "Hnodes".
+        iDestruct (xtchain_snoc_2 with "Hhist Hnew_back_header Hnew_back_next") as "Hhist".
+        iMod (history_update new_back with "Hhistory_auth") as "(Hhistory_auth & #Hhistory_at_new_back)".
+
+        iMod "HΦ" as "(%vs_ & (:model) & _ & HΦ)".
+        iDestruct (model_agree with "Hmodel₁ Hmodel₂") as %->.
+        iMod (model_update (vs ++ [v]) with "Hmodel₁ Hmodel₂") as "(Hmodel₁ & Hmodel₂)".
+        iMod ("HΦ" with "Hmodel₁") as "HΦ".
+
+        iSplitR "HΦ".
+        { iExists (hist ++ [new_back]), past, front, (nodes ++ [new_back]), back, (vs ++ [v]).
+          iSteps; iPureIntro.
+          - rewrite Hhist -assoc //.
+          - set_solver.
+        }
+        iSteps.
+    Qed.
+
+    #[local] Lemma mpsc_queue_1_fix_back_spec t γ i back j new_back :
+      {{{
+        inv' t γ ∗
+        history_at γ i back ∗
+        node_model γ new_back j
+      }}}
+        mpsc_queue_1_fix_back #t #back #new_back
+      {{{
+        RET ();
+        True
+      }}}.
+    Proof.
+      iIntros "%Φ (#Hinv & #Hhistory_at_back & (:node_model =new_back)) HΦ".
+
+      iLöb as "HLöb" forall (i back) "Hhistory_at_back".
+
+      wp_rec. wp_match.
+
+      wp_bind (_ and _)%E.
+      wp_apply (wp_wand itype_bool) as (res) "(%b & ->)".
+      { wp_smart_apply (next_spec new_back with "[$]") as (res) "[-> | (%new_back' & -> & (:node_model =new_back'))]"; last iSteps.
+        wp_pures.
+
+        wp_bind (CAS _ _ _).
+        iInv "Hinv" as "(:inv_inner =1)".
+        wp_cas as _ | [= ->]; first iSteps.
+        iDestruct (history_at_lookup with "Hhistory_auth Hhistory_at_new_back") as %Hnew_back%list_elem_of_lookup_2.
+        iSteps.
+      }
+
+      destruct b; last iSteps.
+      wp_smart_apply domain_yield_spec.
+      wp_smart_apply (back_spec with "Hinv") as (back' i') "(:node_model =back')".
+      iApply ("HLöb" with "HΦ Hhistory_at_back'").
+    Qed.
+
+    Lemma mpsc_queue_1_push_spec t γ ι v :
+      <<<
+        mpsc_queue_1_inv t γ ι
+      | ∀∀ vs,
+        mpsc_queue_1_model γ vs
+      >>>
+        mpsc_queue_1_push #t v @ ↑ι
+      <<<
+        mpsc_queue_1_model γ (vs ++ [v])
+      | RET ();
+        True
+      >>>.
+    Proof.
+      iIntros "%Φ (:inv) HΦ".
+
+      wp_rec.
+      wp_block new_back as "#Hnew_back_header" "_" "(Hnew_back_next & Hnew_back_data & _)".
+      wp_match.
+      wp_smart_apply (back_spec with "Hinv") as (back i) "(:node_model =back)".
+      wp_smart_apply (mpsc_queue_1_push_0_spec with "[$]").
+      iApply (atomic_update_wand with "HΦ"). iIntros "%vs HΦ (%j & #Hhistory_at_new_back)".
+      wp_smart_apply (mpsc_queue_1_fix_back_spec with "[] HΦ"); first iSteps.
+    Qed.
+
+    #[local] Lemma mpsc_queue_1_pop_spec_aux t γ :
+      <<<
+        inv' t γ ∗
+        consumer_2 t
+      | ∀∀ vs,
+        model₁ γ vs
+      >>>
+        mpsc_queue_1_pop #t @ ↑γ.(mpsc_queue_1_name_inv)
+      <<<
+        model₁ γ (tail vs)
+      | RET head vs;
+        consumer_2 t
+      >>>.
+    Proof.
+      iIntros "%Φ (#Hinv & (:consumer_2)) HΦ".
+
+      iLöb as "HLöb".
+
+      iMod (inv_inner_history_at with "Hinv Hconsumer") as "(%i & Hconsumer & (:node_model =front))".
+
+      wp_rec. wp_load. wp_match.
+      wp_smart_apply (next_spec_pop (λ o, _ -∗ Φ o)%I with "[$]") as (res) "(Hconsumer & [(-> & HΦ) | (%new_front & -> & (:node_model =new_front) & HΦ)])"; first iSteps.
+      wp_match. wp_pures.
+
+      wp_bind (_ <-{front} _)%E.
+      iInv "Hinv" as "(:inv_inner =1)".
+      iDestruct (pointsto_agree with "Ht_front Hconsumer") as %[= ->].
+      iCombine "Ht_front Hconsumer" as "Ht_front".
+      rewrite Qp.quarter_three_quarter.
+      wp_store.
+      iEval (rewrite -Qp.quarter_three_quarter) in "Ht_front".
+      iDestruct "Ht_front" as "(Ht_front & Hconsumer)".
+      iDestruct (history_at_lookup with "Hhistory_auth Hhistory_at_front") as %Hlookup.
+      iDestruct (history_at_lookup with "Hhistory_auth Hhistory_at_new_front") as %Hlookup_new.
+      iAssert ⌜length past1 = i⌝%I as %Hpast1_length.
+      { iDestruct (xtchain_NoDup with "Hhist") as %Hnodup.
+        iPureIntro. eapply NoDup_lookup; try done.
+        rewrite Hhist1 list_lookup_middle //.
+      }
+      rewrite Hhist1 (assoc _ _ [_]) lookup_app_r length_app /= in Hlookup_new; first lia.
+      rewrite Nat.add_1_r Hpast1_length Nat.sub_diag in Hlookup_new.
+      destruct nodes1 as [| node nodes1]; first done. injection Hlookup_new as ->.
+      rewrite (assoc _ _ [_]) in Hhist1.
+      iDestruct (big_sepL2_cons_inv_l with "Hnodes") as "(%v & %vs' & -> & Hnew_front_data & Hnodes)".
+
+      iMod "HΦ" as "(%vs & Hmodel₁ & _ & HΦ)".
+      iDestruct (model_agree with "Hmodel₁ Hmodel₂") as %->.
+      iMod (model_update vs' with "Hmodel₁ Hmodel₂") as "(Hmodel₁ & Hmodel₂)".
+      iMod ("HΦ" with "Hmodel₁") as "HΦ".
+
+      iSplitR "Hconsumer Hnew_front_data HΦ". { iFrameSteps. }
+      iSteps.
+    Qed.
+    Lemma mpsc_queue_1_pop_spec t γ ι :
+      <<<
+        mpsc_queue_1_inv t γ ι ∗
+        mpsc_queue_1_consumer t
+      | ∀∀ vs,
+        mpsc_queue_1_model γ vs
+      >>>
+        mpsc_queue_1_pop #t @ ↑ι
+      <<<
+        mpsc_queue_1_model γ (tail vs)
+      | RET head vs;
+        mpsc_queue_1_consumer t
+      >>>.
+    Proof.
+      iIntros "%Φ ((:inv) & (:consumer)) HΦ".
+
+      wp_apply (mpsc_queue_1_pop_spec_aux with "[$]").
+      iAuIntro.
+      iApply (aacc_aupd_commit with "HΦ"); first done. iIntros "%vs (:model)".
+      iAaccIntro with "Hmodel₁"; iSteps.
+    Qed.
+  End mpsc_queue_1_G.
+
+  #[global] Opaque mpsc_queue_1_inv.
+  #[global] Opaque mpsc_queue_1_model.
+  #[global] Opaque mpsc_queue_1_consumer.
+End base.
+
+From zoo_saturn Require
+  mpsc_queue_1__opaque.
+
 Section mpsc_queue_1_G.
   Context `{mpsc_queue_1_G : MpscQueue1G Σ}.
 
-  Record metadata := {
-    metadata_inv : namespace ;
-    metadata_history : gname ;
-    metadata_model : gname ;
-  }.
-  Implicit Type γ : metadata.
+  Implicit Types 𝑡 : location.
+  Implicit Types t : val.
 
-  #[local] Instance metadata_eq_dec : EqDecision metadata :=
-    ltac:(solve_decision).
-  #[local] Instance metadata_countable :
-    Countable metadata.
-  Proof.
-    solve_countable.
-  Qed.
-
-  #[local] Definition history_auth' γ_history hist :=
-    mono_list_auth γ_history (DfracOwn 1) hist.
-  #[local] Definition history_auth γ hist :=
-    history_auth' γ.(metadata_history) hist.
-  #[local] Definition history_at γ i node :=
-    mono_list_at γ.(metadata_history) i node.
-
-  #[local] Definition model₁' γ_model vs :=
-    twins_twin1 γ_model (DfracOwn 1) vs.
-  #[local] Definition model₁ γ vs :=
-    model₁' γ.(metadata_model) vs.
-  #[local] Definition model₂' γ_model vs :=
-    twins_twin2 γ_model vs.
-  #[local] Definition model₂ γ vs :=
-    model₂' γ.(metadata_model) vs.
-
-  #[local] Definition node_model γ node i : iProp Σ :=
-    node ↦ₕ Header §Node 2 ∗
-    history_at γ i node.
-  #[local] Instance : CustomIpatFormat "node_model" :=
-    " ( #H{}_header &
-        #Hhistory_at_{}
-      )
-    ".
-
-  #[local] Definition inv_inner l γ : iProp Σ :=
-    ∃ hist past front nodes back vs,
-    ⌜hist = past ++ front :: nodes⌝ ∗
-    ⌜back ∈ hist⌝ ∗
-    l.[front] ↦{#1/4} #front ∗
-    l.[back] ↦ #back ∗
-    xtchain (Header §Node 2) (DfracOwn 1) hist §Null ∗
-    ([∗ list] node; v ∈ nodes; vs, node.[data] ↦ v) ∗
-    history_auth γ hist ∗
-    model₂ γ vs.
-  #[local] Instance : CustomIpatFormat "inv_inner" :=
-    " ( %hist{} &
-        %past{} &
-        %front{} &
-        %nodes{} &
-        %back{} &
-        %vs{} &
-        >%Hhist{} &
-        >%Hback{} &
-        >Hl_front &
-        >Hl_back &
-        >Hhist &
-        >Hnodes &
-        >Hhistory_auth &
-        >Hmodel₂
-      )
-    ".
-  #[local] Definition inv' l γ :=
-    inv γ.(metadata_inv) (inv_inner l γ).
   Definition mpsc_queue_1_inv t ι : iProp Σ :=
-    ∃ l γ,
-    ⌜t = #l⌝ ∗
-    ⌜ι = γ.(metadata_inv)⌝ ∗
-    meta l nroot γ ∗
-    inv' l γ.
+    ∃ 𝑡 γ,
+    ⌜t = #𝑡⌝ ∗
+    meta 𝑡 nroot γ ∗
+    base.mpsc_queue_1_inv 𝑡 γ ι.
   #[local] Instance : CustomIpatFormat "inv" :=
-    " ( %l &
-        %γ &
-        -> &
-        -> &
-        #Hmeta &
-        #Hinv
+    " ( %𝑡{} &
+        %γ{} &
+        {%Heq{};->} &
+        #Hmeta{_{}} &
+        Hinv{_{}}
       )
     ".
 
   Definition mpsc_queue_1_model t vs : iProp Σ :=
-    ∃ l γ,
-    ⌜t = #l⌝ ∗
-    meta l nroot γ ∗
-    model₁ γ vs.
+    ∃ 𝑡 γ,
+    ⌜t = #𝑡⌝ ∗
+    meta 𝑡 nroot γ ∗
+    base.mpsc_queue_1_model γ vs.
   #[local] Instance : CustomIpatFormat "model" :=
-    " ( %l{;_} &
-        %γ{;_} &
-        %Heq{} &
-        #Hmeta_{} &
-        Hmodel₁{_{}}
+    " ( %𝑡{} &
+        %γ{} &
+        {%Heq{};->} &
+        #Hmeta{_{}} &
+        Hmodel{_{}}
       )
     ".
 
-  #[local] Definition consumer_1 l front : iProp Σ :=
-    l.[front] ↦{#3/4} #front.
-  #[local] Definition consumer_2 l : iProp Σ :=
-    ∃ front,
-    consumer_1 l front.
-  #[local] Instance : CustomIpatFormat "consumer_2" :=
-    " ( %front{} &
-        Hconsumer{_{}}
-      )
-    ".
   Definition mpsc_queue_1_consumer t : iProp Σ :=
-    ∃ l,
-    ⌜t = #l⌝ ∗
-    consumer_2 l.
+    ∃ 𝑡,
+    ⌜t = #𝑡⌝ ∗
+    base.mpsc_queue_1_consumer 𝑡.
   #[local] Instance : CustomIpatFormat "consumer" :=
-    " ( %l{;_} &
-        %Heq{} &
-        (:consumer_2 {//})
+    " ( %𝑡{} &
+        {%Heq{};->} &
+        Hconsumer{_{}}
       )
     ".
 
@@ -186,88 +860,6 @@ Section mpsc_queue_1_G.
     apply _.
   Qed.
 
-  #[local] Lemma history_alloc front :
-    ⊢ |==>
-      ∃ γ_history,
-      history_auth' γ_history [front].
-  Proof.
-    apply mono_list_alloc.
-  Qed.
-  #[local] Lemma history_at_get {γ hist} i node :
-    hist !! i = Some node →
-    history_auth γ hist ⊢
-    history_at γ i node.
-  Proof.
-    apply mono_list_at_get.
-  Qed.
-  #[local] Lemma history_at_lookup γ hist i node :
-    history_auth γ hist -∗
-    history_at γ i node -∗
-    ⌜hist !! i = Some node⌝.
-  Proof.
-    apply mono_list_at_valid.
-  Qed.
-  #[local] Lemma history_update {γ hist} node :
-    history_auth γ hist ⊢ |==>
-      history_auth γ (hist ++ [node]) ∗
-      history_at γ (length hist) node.
-  Proof.
-    iIntros "Hauth".
-    iMod (mono_list_update_snoc with "Hauth") as "Hauth".
-    iDestruct (history_at_get with "Hauth") as "#Hat".
-    { rewrite lookup_snoc_Some. naive_solver. }
-    iSteps.
-  Qed.
-
-  #[local] Lemma model_alloc :
-    ⊢ |==>
-      ∃ γ_model,
-      model₁' γ_model [] ∗
-      model₂' γ_model [].
-  Proof.
-    apply twins_alloc'.
-  Qed.
-  #[local] Lemma model₁_exclusive γ vs1 vs2 :
-    model₁ γ vs1 -∗
-    model₁ γ vs2 -∗
-    False.
-  Proof.
-    apply twins_twin1_exclusive.
-  Qed.
-  #[local] Lemma model_agree γ vs1 vs2 :
-    model₁ γ vs1 -∗
-    model₂ γ vs2 -∗
-    ⌜vs1 = vs2⌝.
-  Proof.
-    apply: twins_agree_L.
-  Qed.
-  #[local] Lemma model_update {γ vs1 vs2} vs :
-    model₁ γ vs1 -∗
-    model₂ γ vs2 ==∗
-      model₁ γ vs ∗
-      model₂ γ vs.
-  Proof.
-    apply twins_update.
-  Qed.
-
-  #[local] Lemma inv_inner_history_at l γ front :
-    inv' l γ -∗
-    consumer_1 l front ={⊤}=∗
-      ∃ i,
-      consumer_1 l front ∗
-      node_model γ front i.
-  Proof.
-    iIntros "#Hinv Hconsumer".
-    iInv "Hinv" as "(:inv_inner =1)".
-    iDestruct (pointsto_agree with "Hl_front Hconsumer") as %[= ->].
-    assert (hist1 !! (length past1) = Some front) as Hlookup.
-    { rewrite Hhist1 list_lookup_middle //. }
-    iDestruct (xtchain_lookup_header with "Hhist") as "#Hfront_header"; first done.
-    iDestruct (history_at_get (length past1) front with "Hhistory_auth") as "#Hhistory_at_front"; first done.
-    iSplitR "Hconsumer". { iFrameSteps. }
-    iSteps.
-  Qed.
-
   Lemma mpsc_queue_1_model_exclusive t vs1 vs2 :
     mpsc_queue_1_model t vs1 -∗
     mpsc_queue_1_model t vs2 -∗
@@ -275,7 +867,7 @@ Section mpsc_queue_1_G.
   Proof.
     iIntros "(:model =1) (:model =2)". simplify.
     iDestruct (meta_agree with "Hmeta_1 Hmeta_2") as %->.
-    iApply (model₁_exclusive with "Hmodel₁_1 Hmodel₁_2").
+    iApply (base.mpsc_queue_1_model_exclusive with "Hmodel_1 Hmodel_2").
   Qed.
 
   Lemma mpsc_queue_1_consumer_exclusive t :
@@ -284,7 +876,7 @@ Section mpsc_queue_1_G.
     False.
   Proof.
     iIntros "(:consumer =1) (:consumer =2)". simplify.
-    iDestruct (pointsto_dfrac_ne with "Hconsumer_1 Hconsumer_2") as %?; naive_solver.
+    iApply (base.mpsc_queue_1_consumer_exclusive with "Hconsumer_1 Hconsumer_2").
   Qed.
 
   Lemma mpsc_queue_1_create_spec ι :
@@ -301,297 +893,10 @@ Section mpsc_queue_1_G.
   Proof.
     iIntros "%Φ _ HΦ".
 
-    wp_rec.
-    wp_block front as "#Hfront_header" "_" "(Hfront_next & _)".
-    wp_block l as "Hmeta" "(Hl_front & Hl_back & _)".
-    iEval (rewrite -Qp.quarter_three_quarter) in "Hl_front".
-    iDestruct "Hl_front" as "(Hl_front & Hconsumer)".
-
-    iMod history_alloc as "(%γ_history & Hhistory_auth)".
-    iMod model_alloc as "(%γ_model & Hmodel₁ & Hmodel₂)".
-
-    pose γ := {|
-      metadata_inv := ι ;
-      metadata_history := γ_history ;
-      metadata_model := γ_model ;
-    |}.
-
-    iMod (meta_set γ with "Hmeta") as "#Hmeta"; first done.
-
-    iApply "HΦ".
-    iSplitR "Hmodel₁ Hconsumer"; last iFrameSteps.
-    iExists l, γ. iStep 3. iApply inv_alloc.
-    iExists [front], [], front, [], front, []. iFrameSteps.
-    - rewrite list_elem_of_singleton //.
-    - rewrite xtchain_singleton. iSteps.
-  Qed.
-
-  #[local] Lemma mpsc_queue_1_front_spec l γ :
-    {{{
-      inv' l γ
-    }}}
-      (#l).{front}
-    {{{ front i,
-      RET #front;
-      node_model γ front i
-    }}}.
-  Proof.
-    iIntros "%Φ #Hinv HΦ".
-
-    iInv "Hinv" as "(:inv_inner)".
-    wp_load.
-    assert (hist !! (length past) = Some front) as Hlookup.
-    { rewrite Hhist list_lookup_middle //. }
-    iDestruct (xtchain_lookup_header with "Hhist") as "#Hfront_header"; first done.
-    iDestruct (history_at_get _ front with "Hhistory_auth") as "#Hhistory_at_front"; first done.
-    iSplitR "HΦ". { iFrameSteps. }
+    iApply wp_fupd.
+    wp_apply (base.mpsc_queue_1_create_spec with "[//]") as (𝑡 γ) "(Hmeta & Hinv & Hmodel & Hconsumer)".
+    iMod (meta_set γ with "Hmeta"); first done.
     iSteps.
-  Qed.
-
-  #[local] Lemma back_spec l γ :
-    {{{
-      inv' l γ
-    }}}
-      (#l).{back}
-    {{{ back i,
-      RET #back;
-      node_model γ back i
-    }}}.
-  Proof.
-    iIntros "%Φ #Hinv HΦ".
-
-    iInv "Hinv" as "(:inv_inner)".
-    wp_load.
-    pose proof Hback as (i & Hlookup)%list_elem_of_lookup.
-    iDestruct (xtchain_lookup_header with "Hhist") as "#Hback_header"; first done.
-    iDestruct (history_at_get with "Hhistory_auth") as "#Hhistory_at_back"; first done.
-    iSplitR "HΦ". { iFrameSteps. }
-    iSteps.
-  Qed.
-
-  Inductive operation :=
-    | IsEmpty (Ψ : bool → iProp Σ)
-    | Pop (Ψ : option val → iProp Σ)
-    | Other.
-  Implicit Types op : operation.
-  Inductive operation' :=
-    | IsEmpty'
-    | Pop'
-    | Other'.
-  #[local] Instance operation'_eq_dec : EqDecision operation' :=
-    ltac:(solve_decision).
-  #[local] Coercion operation_to_operation' op :=
-    match op with
-    | IsEmpty _ =>
-        IsEmpty'
-    | Pop _ =>
-        Pop'
-    | Other =>
-        Other'
-    end.
-  #[local] Definition is_empty_au l γ (Ψ : bool → iProp Σ) : iProp Σ :=
-    AU <{
-      ∃∃ vs,
-      mpsc_queue_1_model #l vs
-    }> @ ⊤ ∖ ↑γ.(metadata_inv), ∅ <{
-      mpsc_queue_1_model #l vs
-    , COMM
-      Ψ (bool_decide (vs = []))
-    }>.
-  #[local] Definition pop_au γ (Ψ : option val → iProp Σ) : iProp Σ :=
-    AU <{
-      ∃∃ vs,
-      model₁ γ vs
-    }> @ ⊤ ∖ ↑γ.(metadata_inv), ∅ <{
-      model₁ γ (tail vs)
-    , COMM
-      Ψ (head vs)
-    }>.
-  #[local] Lemma next_spec_aux op l γ i node :
-    {{{
-      meta l nroot γ ∗
-      inv' l γ ∗
-      history_at γ i node ∗
-      ( if decide (op = Other' :> operation') then True else
-          consumer_1 l node
-      ) ∗
-      match op with
-      | IsEmpty Ψ =>
-          is_empty_au l γ Ψ
-      | Pop Ψ =>
-          pop_au γ Ψ
-      | Other =>
-          True
-      end
-    }}}
-      (#node).{next}
-    {{{ res,
-      RET res;
-      ( if decide (op = Other' :> operation') then True else
-          consumer_1 l node
-      ) ∗
-      ( ⌜res = §Null%V⌝ ∗
-        match op with
-        | IsEmpty Ψ =>
-            Ψ true
-        | Pop Ψ =>
-            Ψ None
-        | Other =>
-            True
-        end
-      ∨ ∃ node',
-        ⌜res = #node'⌝ ∗
-        node_model γ node' (S i) ∗
-        match op with
-        | IsEmpty Ψ =>
-            Ψ false
-        | Pop Ψ =>
-            pop_au γ Ψ
-        | Other =>
-            True
-        end
-      )
-    }}}.
-  Proof.
-    iIntros "%Φ (#Hmeta & #Hinv & #Hhistory_at_node & Hop) HΦ".
-
-    iInv "Hinv" as "(:inv_inner)".
-    iDestruct (history_at_lookup with "Hhistory_auth Hhistory_at_node") as %Hlookup.
-    iDestruct (xtchain_lookup_acc with "Hhist") as "(_ & Hnode & Hhist)"; first done.
-    wp_load.
-    iDestruct ("Hhist" with "Hnode") as "Hhist".
-    destruct (hist !! S i) as [node' |] eqn:Hlookup'; simpl.
-
-    - iDestruct (xtchain_lookup_header with "Hhist") as "#Hnode'_header"; first done.
-      iDestruct (history_at_get (S i) with "Hhistory_auth") as "#Hhistory_at_node'"; first done.
-      destruct op; [| iFrameSteps..].
-      iDestruct "Hop" as "(Hconsumer & HΨ)".
-      iDestruct (pointsto_agree with "Hl_front Hconsumer") as %[= <-].
-
-      iMod "HΨ" as "(%vs_ & (:model) & _ & HΨ)". injection Heq as <-.
-      iDestruct (meta_agree with "Hmeta Hmeta_") as %<-. iClear "Hmeta_".
-      iDestruct (model_agree with "Hmodel₁ Hmodel₂") as %->.
-      iMod ("HΨ" with "[Hmodel₁]") as "HΨ"; first iSteps.
-
-      iAssert ⌜length past = i⌝%I as %Hpast_length.
-      { iDestruct (xtchain_NoDup with "Hhist") as %Hnodup.
-        iPureIntro. eapply NoDup_lookup; try done.
-        rewrite Hhist list_lookup_middle //.
-      }
-      rewrite -(bool_decide_ext _ _ (length_zero_iff_nil _)).
-      iDestruct (big_sepL2_length with "Hnodes") as %<-.
-      rewrite bool_decide_eq_false_2.
-      { apply (f_equal length) in Hhist as Hhist_length.
-        simpl_length/= in Hhist_length.
-        apply lookup_lt_Some in Hlookup'.
-        lia.
-      }
-
-      iSplitR "Hconsumer HΨ HΦ". { iFrameSteps. }
-      iSteps.
-
-    - destruct_decide (op = Other' :> operation').
-      { destruct op; try done. iSteps. }
-      iDestruct "Hop" as "(Hconsumer & HΨ)".
-      iDestruct (pointsto_agree with "Hl_front Hconsumer") as %[= <-].
-
-      iAssert ⌜length past = i⌝%I as %Hpast_length.
-      { iDestruct (xtchain_NoDup with "Hhist") as %Hnodup.
-        iPureIntro. eapply NoDup_lookup; try done.
-        rewrite Hhist list_lookup_middle //.
-      }
-      destruct_decide (length vs = 0) as ->%nil_length_inv | Hvs; last first.
-      { iDestruct (big_sepL2_length with "Hnodes") as %?.
-        exfalso.
-        apply (f_equal length) in Hhist.
-        opose proof* length_lookup_last as Heq; [done.. |].
-        simpl_length/= in Hhist. lia.
-      }
-
-      destruct op; last done.
-
-      + iMod "HΨ" as "(%vs & (:model) & _ & HΨ)". injection Heq as <-.
-        iDestruct (meta_agree with "Hmeta Hmeta_") as %<-. iClear "Hmeta_".
-        iDestruct (model_agree with "Hmodel₁ Hmodel₂") as %->.
-        iMod ("HΨ" with "[Hmodel₁]") as "HΨ"; first iSteps.
-
-        iSplitR "Hconsumer HΨ HΦ". { iFrameSteps. }
-        iSteps.
-
-      + iMod "HΨ" as "(%vs & Hmodel₁ & _ & HΨ)".
-        iDestruct (model_agree with "Hmodel₁ Hmodel₂") as %->.
-        iMod ("HΨ" with "Hmodel₁") as "HΨ".
-
-        iSplitR "Hconsumer HΨ HΦ". { iFrameSteps. }
-        iSteps.
-  Qed.
-  #[local] Lemma next_spec {l γ i} node :
-    {{{
-      meta l nroot γ ∗
-      inv' l γ ∗
-      history_at γ i node
-    }}}
-      (#node).{next}
-    {{{ res,
-      RET res;
-        ⌜res = §Null%V⌝
-      ∨ ∃ node',
-        ⌜res = #node'⌝ ∗
-        node_model γ node' (S i)
-    }}}.
-  Proof.
-    iIntros "%Φ (#Hmeta & #Hinv & #Hhistory_at_node) HΦ".
-    wp_apply (next_spec_aux Other); iSteps.
-  Qed.
-  #[local] Lemma next_spec_is_empty {l γ i node} Ψ :
-    {{{
-      meta l nroot γ ∗
-      inv' l γ ∗
-      history_at γ i node ∗
-      consumer_1 l node ∗
-      is_empty_au l γ Ψ
-    }}}
-      (#node).{next}
-    {{{ res,
-      RET res;
-      consumer_1 l node ∗
-      ( ⌜res = §Null%V⌝ ∗
-        Ψ true
-      ∨ ∃ node',
-        ⌜res = #node'⌝ ∗
-        node_model γ node' (S i) ∗
-        Ψ false
-      )
-    }}}.
-  Proof.
-    iIntros "%Φ (#Hmeta & #Hinv & #Hhistory_at_node & Hl_front & Hau) HΦ".
-    wp_apply (next_spec_aux (IsEmpty _) with "[$]").
-    iFrameSteps.
-  Qed.
-  #[local] Lemma next_spec_pop {l γ i node} Ψ :
-    {{{
-      meta l nroot γ ∗
-      inv' l γ ∗
-      history_at γ i node ∗
-      consumer_1 l node ∗
-      pop_au γ Ψ
-    }}}
-      (#node).{next}
-    {{{ res,
-      RET res;
-      consumer_1 l node ∗
-      ( ⌜res = §Null%V⌝ ∗
-        Ψ None
-      ∨ ∃ node',
-        ⌜res = #node'⌝ ∗
-        node_model γ node' (S i) ∗
-        pop_au γ Ψ
-      )
-    }}}.
-  Proof.
-    iIntros "%Φ (#Hmeta & #Hinv & #Hhistory_at_node & Hl_front & Hau) HΦ".
-    wp_apply (next_spec_aux (Pop _) with "[$]").
-    iFrameSteps.
   Qed.
 
   Lemma mpsc_queue_1_is_empty_spec t ι :
@@ -608,112 +913,13 @@ Section mpsc_queue_1_G.
       mpsc_queue_1_consumer t
     >>>.
   Proof.
-    iIntros "%Φ ((:inv) & (:consumer)) HΦ". injection Heq as <-.
+    iIntros "%Φ ((:inv =1) & (:consumer =2)) HΦ". simplify.
 
-    iMod (inv_inner_history_at with "Hinv Hconsumer") as "(%i & Hl_front & #Hfront_header & #Hhistory_at_front)".
-
-    wp_rec. wp_load. wp_match.
-    wp_smart_apply (next_spec_is_empty (λ b, _ -∗ Φ #b)%I with "[$]").
-    iSteps.
-  Qed.
-
-  #[local] Lemma mpsc_queue_1_push_0_spec l γ i node new_back v :
-    <<<
-      meta l nroot γ ∗
-      inv' l γ ∗
-      node_model γ node i ∗
-      new_back ↦ₕ Header §Node 2 ∗
-      new_back.[next] ↦ §Null ∗
-      new_back.[data] ↦ v
-    | ∀∀ vs,
-      mpsc_queue_1_model #l vs
-    >>>
-      mpsc_queue_1_push_0 #node #new_back @ ↑γ.(metadata_inv)
-    <<<
-      mpsc_queue_1_model #l (vs ++ [v])
-    | RET ();
-      ∃ j,
-      history_at γ j new_back
-    >>>.
-  Proof.
-    iIntros "%Φ (#Hmeta & #Hinv & (:node_model =node) & #Hnew_back_header & Hnew_back_next & Hnew_back_data) HΦ".
-
-    iLöb as "HLöb" forall (i node) "Hnode_header Hhistory_at_node".
-
-    wp_rec. wp_match.
-    wp_smart_apply (next_spec with "[$]") as (res) "[-> | (%node' & -> & (:node_model =node'))]"; last iSteps.
-    wp_pures.
-
-    wp_bind (CAS _ _ _).
-    iInv "Hinv" as "(:inv_inner)".
-    iDestruct (history_at_lookup with "Hhistory_auth Hhistory_at_node") as %Hlookup.
-    iDestruct (xtchain_lookup with "Hhist") as "(Hhist1 & _ & Hnode & Hhist2)"; first done.
-    destruct (hist !! S i) as [node' |] eqn:Hlookup'; simpl.
-
-    - wp_cas as _ | [=].
-      iDestruct (xtchain_lookup_2 with "Hhist1 Hnode_header Hnode Hhist2") as "Hhist"; [done | rewrite Hlookup' // |].
-      iSplitR "Hnew_back_next Hnew_back_data HΦ". { iFrameSteps. }
-      iSteps.
-
-    - wp_cas as ? | _; first done.
-      iDestruct (xtchain_lookup_2 with "Hhist1 Hnode_header Hnode []") as "Hhist"; [done | rewrite Hlookup' // | ..].
-      { rewrite -(length_lookup_last hist i) // drop_all.
-        iApply xtchain_nil.
-      }
-      iDestruct (big_sepL2_snoc_2 with "Hnodes Hnew_back_data") as "Hnodes".
-      iDestruct (xtchain_snoc_2 with "Hhist Hnew_back_header Hnew_back_next") as "Hhist".
-      iMod (history_update new_back with "Hhistory_auth") as "(Hhistory_auth & #Hhistory_at_new_back)".
-
-      iMod "HΦ" as "(%vs_ & (:model) & _ & HΦ)". injection Heq as <-.
-      iDestruct (meta_agree with "Hmeta Hmeta_") as %<-. iClear "Hmeta_".
-      iDestruct (model_agree with "Hmodel₁ Hmodel₂") as %->.
-      iMod (model_update (vs ++ [v]) with "Hmodel₁ Hmodel₂") as "(Hmodel₁ & Hmodel₂)".
-      iMod ("HΦ" with "[Hmodel₁]") as "HΦ"; [iSteps.. |].
-
-      iSplitR "HΦ".
-      { iExists (hist ++ [new_back]), past, front, (nodes ++ [new_back]), back, (vs ++ [v]).
-        iSteps; iPureIntro.
-        - rewrite Hhist -assoc //.
-        - set_solver.
-      }
-      iSteps.
-  Qed.
-
-  #[local] Lemma mpsc_queue_1_fix_back_spec l γ i back j new_back :
-    {{{
-      meta l nroot γ ∗
-      inv' l γ ∗
-      history_at γ i back ∗
-      node_model γ new_back j
-    }}}
-      mpsc_queue_1_fix_back #l #back #new_back
-    {{{
-      RET ();
-      True
-    }}}.
-  Proof.
-    iIntros "%Φ (#Hmeta & #Hinv & #Hhistory_at_back & (:node_model =new_back)) HΦ".
-
-    iLöb as "HLöb" forall (i back) "Hhistory_at_back".
-
-    wp_rec. wp_match.
-
-    wp_bind (_ and _)%E.
-    wp_apply (wp_wand itype_bool) as (res) "(%b & ->)".
-    { wp_smart_apply (next_spec new_back with "[$]") as (res) "[-> | (%new_back' & -> & (:node_model =new_back'))]"; last iSteps.
-      wp_pures.
-
-      wp_bind (CAS _ _ _).
-      iInv "Hinv" as "(:inv_inner =1)".
-      wp_cas as _ | [= ->]; first iSteps.
-      iDestruct (history_at_lookup with "Hhistory_auth Hhistory_at_new_back") as %Hnew_back%list_elem_of_lookup_2.
-      iSteps.
+    awp_apply (base.mpsc_queue_1_is_empty_spec with "[$]").
+    { iApply (aacc_aupd_commit with "HΦ"); first done. iIntros "%vs (:model =3)". simplify.
+      iDestruct (meta_agree with "Hmeta_1 Hmeta_3") as %->. iClear "Hmeta_1".
+      iAaccIntro with "Hmodel_3"; iSteps.
     }
-
-    destruct b; last iSteps.
-    wp_smart_apply domain_yield_spec.
-    wp_smart_apply (back_spec with "Hinv") as (back' i') "(:node_model =back')".
-    iApply ("HLöb" with "HΦ Hhistory_at_back'").
   Qed.
 
   Lemma mpsc_queue_1_push_spec t ι v :
@@ -731,69 +937,13 @@ Section mpsc_queue_1_G.
   Proof.
     iIntros "%Φ (:inv) HΦ".
 
-    wp_rec.
-    wp_block new_back as "#Hnew_back_header" "_" "(Hnew_back_next & Hnew_back_data & _)".
-    wp_match.
-    wp_smart_apply (back_spec with "Hinv") as (back i) "(:node_model =back)".
-    wp_smart_apply (mpsc_queue_1_push_0_spec with "[$]").
-    iApply (atomic_update_wand with "HΦ"). iIntros "%vs HΦ (%j & #Hhistory_at_new_back)".
-    wp_smart_apply (mpsc_queue_1_fix_back_spec with "[] HΦ"); first iSteps.
-  Qed.
-
-  #[local] Lemma mpsc_queue_1_pop_spec_aux l γ :
-    <<<
-      meta l nroot γ ∗
-      inv' l γ ∗
-      consumer_2 l
-    | ∀∀ vs,
-      model₁ γ vs
-    >>>
-      mpsc_queue_1_pop #l @ ↑γ.(metadata_inv)
-    <<<
-      model₁ γ (tail vs)
-    | RET head vs;
-      consumer_2 l
-    >>>.
-  Proof.
-    iIntros "%Φ (#Hmeta & #Hinv & (:consumer_2)) HΦ".
-
-    iLöb as "HLöb".
-
-    iMod (inv_inner_history_at with "Hinv Hconsumer") as "(%i & Hconsumer & (:node_model =front))".
-
-    wp_rec. wp_load. wp_match.
-    wp_smart_apply (next_spec_pop (λ o, _ -∗ Φ o)%I with "[$]") as (res) "(Hconsumer & [(-> & HΦ) | (%new_front & -> & (:node_model =new_front) & HΦ)])"; first iSteps.
-    wp_match. wp_pures.
-
-    wp_bind (_ <-{front} _)%E.
-    iInv "Hinv" as "(:inv_inner =1)".
-    iDestruct (pointsto_agree with "Hl_front Hconsumer") as %[= ->].
-    iCombine "Hl_front Hconsumer" as "Hl_front".
-    rewrite Qp.quarter_three_quarter.
-    wp_store.
-    iEval (rewrite -Qp.quarter_three_quarter) in "Hl_front".
-    iDestruct "Hl_front" as "(Hl_front & Hconsumer)".
-    iDestruct (history_at_lookup with "Hhistory_auth Hhistory_at_front") as %Hlookup.
-    iDestruct (history_at_lookup with "Hhistory_auth Hhistory_at_new_front") as %Hlookup_new.
-    iAssert ⌜length past1 = i⌝%I as %Hpast1_length.
-    { iDestruct (xtchain_NoDup with "Hhist") as %Hnodup.
-      iPureIntro. eapply NoDup_lookup; try done.
-      rewrite Hhist1 list_lookup_middle //.
+    awp_apply (base.mpsc_queue_1_push_spec with "[$]").
+    { iApply (aacc_aupd_commit with "HΦ"); first done. iIntros "%vs (:model =1)". simplify.
+      iDestruct (meta_agree with "Hmeta Hmeta_1") as %<-. iClear "Hmeta_1".
+      iAaccIntro with "Hmodel_1"; iSteps.
     }
-    rewrite Hhist1 (assoc _ _ [_]) lookup_app_r length_app /= in Hlookup_new; first lia.
-    rewrite Nat.add_1_r Hpast1_length Nat.sub_diag in Hlookup_new.
-    destruct nodes1 as [| node nodes1]; first done. injection Hlookup_new as ->.
-    rewrite (assoc _ _ [_]) in Hhist1.
-    iDestruct (big_sepL2_cons_inv_l with "Hnodes") as "(%v & %vs' & -> & Hnew_front_data & Hnodes)".
-
-    iMod "HΦ" as "(%vs & Hmodel₁ & _ & HΦ)".
-    iDestruct (model_agree with "Hmodel₁ Hmodel₂") as %->.
-    iMod (model_update vs' with "Hmodel₁ Hmodel₂") as "(Hmodel₁ & Hmodel₂)".
-    iMod ("HΦ" with "Hmodel₁") as "HΦ".
-
-    iSplitR "Hconsumer Hnew_front_data HΦ". { iFrameSteps. }
-    iSteps.
   Qed.
+
   Lemma mpsc_queue_1_pop_spec t ι :
     <<<
       mpsc_queue_1_inv t ι ∗
@@ -808,18 +958,15 @@ Section mpsc_queue_1_G.
       mpsc_queue_1_consumer t
     >>>.
   Proof.
-    iIntros "%Φ ((:inv) & (:consumer)) HΦ". injection Heq as <-.
+    iIntros "%Φ ((:inv =1) & (:consumer =2)) HΦ". simplify.
 
-    wp_apply (mpsc_queue_1_pop_spec_aux with "[$]").
-    iAuIntro.
-    iApply (aacc_aupd_commit with "HΦ"); first done. iIntros "%vs (:model)". injection Heq as <-.
-    iDestruct (meta_agree with "Hmeta Hmeta_") as %<-.
-    iAaccIntro with "Hmodel₁"; iSteps.
+    awp_apply (base.mpsc_queue_1_pop_spec with "[$]").
+    { iApply (aacc_aupd_commit with "HΦ"); first done. iIntros "%vs (:model =3)". simplify.
+      iDestruct (meta_agree with "Hmeta_1 Hmeta_3") as %->. iClear "Hmeta_1".
+      iAaccIntro with "Hmodel_3"; iSteps.
+    }
   Qed.
 End mpsc_queue_1_G.
-
-From zoo_saturn Require
-  mpsc_queue_1__opaque.
 
 #[global] Opaque mpsc_queue_1_inv.
 #[global] Opaque mpsc_queue_1_model.
